unfinished: new Iface thy

Primitive_Matchers/Iface.thy
@@ -2,61 +2,156 @@ theory Iface
 imports String "../Output_Format/Negation_Type"
 begin
 
+section{*Network Interfaces*}
+
 datatype iface = Iface "string negation_type" | IfaceAny
 
-text{*If the interface name ends in a "+", then any interface which begins with this name will match. (man iptables)*}
-fun cmp_iface_name :: "string \<Rightarrow> string \<Rightarrow> bool" where
-  "cmp_iface_name [] [] \<longleftrightarrow> True" |
-  "cmp_iface_name [i1] [] \<longleftrightarrow> (i1 = CHR ''+'')" |
-  "cmp_iface_name [] [i2] \<longleftrightarrow> (i2 = CHR ''+'')" |
-  "cmp_iface_name [i1] [i2] \<longleftrightarrow> (i1 = CHR ''+'' \<or> i2 = CHR ''+'' \<or> i1 = i2)" |
-  "cmp_iface_name [i1] i2s \<longleftrightarrow> (i1 = CHR ''+'')" |
-  "cmp_iface_name i1s [i2] \<longleftrightarrow> (i2 = CHR ''+'')" |
-  "cmp_iface_name (i1#i1s) (i2#i2s) \<longleftrightarrow> (if i1 = i2 then cmp_iface_name i1s i2s else False)" |
-  "cmp_iface_name _ _ \<longleftrightarrow> False"
+text_raw{*If the interface name ends in a ``+'', then any interface which begins with this name will match. (man iptables)
 
-lemma cmp_iface_name_refl: "cmp_iface_name is is"
+Here is how iptables handles this wildcard on my system. A packet for the loopback interface \texttt{lo} is matched by the following expressions
+\begin{itemize}
+  \item lo
+  \item lo+
+  \item l+
+  \item +
+\end{itemize}
+
+It is not matched by the following expressions
+\begin{itemize}
+  \item lo++
+  \item lo+++
+  \item lo1+
+  \item lo1
+\end{itemize}
+
+By the way: \texttt{Warning: weird character in interface ` ' ('/' and ' ' are not allowed by the kernel).}
+*}
+
+fun iface_name_eq :: "string \<Rightarrow> string \<Rightarrow> bool" where
+  "iface_name_eq [] [] \<longleftrightarrow> True" |
+  "iface_name_eq [i1] [] \<longleftrightarrow> (i1 = CHR ''+'')" |
+  "iface_name_eq [] [i2] \<longleftrightarrow> (i2 = CHR ''+'')" |
+  "iface_name_eq [i1] [i2] \<longleftrightarrow> (i1 = CHR ''+'' \<or> i2 = CHR ''+'' \<or> i1 = i2)" |
+  "iface_name_eq (i1#i1s) (i2#i2s) \<longleftrightarrow> (i1 = CHR ''+'' \<and> i1s = [] \<or> i2 = CHR ''+'' \<and> i2s = []) \<or> (i1 = i2 \<and> iface_name_eq i1s i2s)" |
+  "iface_name_eq _ _ \<longleftrightarrow> False"
+
+
+  lemma "iface_name_eq ''lo'' ''lo''" by eval
+  lemma "iface_name_eq ''lo'' ''lo+''" by eval
+  lemma "iface_name_eq ''lo'' ''l+''" by eval
+  lemma "iface_name_eq ''lo'' ''+''" by eval
+  lemma "\<not> iface_name_eq ''lo'' ''lo++''" by eval
+  lemma "\<not> iface_name_eq ''lo'' ''lo+++''" by eval
+  lemma "\<not> iface_name_eq ''lo'' ''lo1+''" by eval
+  lemma "\<not> iface_name_eq ''lo'' ''lo1''" by eval
+  text{*The wildcard interface name*}
+  lemma "iface_name_eq '''' ''+''" by eval
+
+fun iface_name_is_wildcard :: "string \<Rightarrow> bool" where
+  "iface_name_is_wildcard [] \<longleftrightarrow> False" |
+  "iface_name_is_wildcard [s] \<longleftrightarrow> s = CHR ''+''" |
+  "iface_name_is_wildcard (_#ss) \<longleftrightarrow> iface_name_is_wildcard ss"
+lemma "iface_name_is_wildcard eth \<longleftrightarrow> (case rev eth of [] \<Rightarrow> False | s#ss \<Rightarrow> s = CHR ''+'')"
+  apply(induction eth rule: iface_name_is_wildcard.induct)
+   apply(simp_all)
+  apply(rename_tac s s' ss)
+  apply(case_tac "rev ss")
+   apply(simp)
+  apply(simp)
+  done
+
+
+
+lemma "iface_name_eq i1 i2 \<longleftrightarrow> i1 = i2 \<or>
+      iface_name_is_wildcard i1 \<and> take ((length i1) - 1) i1 = take ((length i1) - 1) i2 \<or>
+      iface_name_is_wildcard i2 \<and> take ((length i2) - 1) i2 = take ((length i2) - 1) i1"
+apply(induction i1 i2 rule: iface_name_eq.induct)
+apply(simp_all)
+apply(auto)[1]
+apply(safe)[1]
+apply(simp_all)
+apply (metis append_take_drop_id hd_append2 iface_name_is_wildcard.simps(2) length_0_conv list.sel(1) take_eq_Nil)
+oops (*TODO*)
+
+lemma iface_name_eq_refl: "iface_name_eq is is"
 proof -
 { fix i1 i2
-  have "i1 = i2 \<Longrightarrow> cmp_iface_name i1 i2"
-    by(induction i1 i2 rule: cmp_iface_name.induct)(auto)
+  have "i1 = i2 \<Longrightarrow> iface_name_eq i1 i2"
+    by(induction i1 i2 rule: iface_name_eq.induct)(auto)
  } thus ?thesis by simp 
 qed
-lemma cmp_iface_name_sym: "cmp_iface_name i1 i2 \<Longrightarrow> cmp_iface_name i2 i1"
-  by(induction i1 i2 rule: cmp_iface_name.induct)(auto split: split_if_asm)
+lemma iface_name_eq_sym: "iface_name_eq i1 i2 \<Longrightarrow> iface_name_eq i2 i1"
+  by(induction i1 i2 rule: iface_name_eq.induct)(auto split: split_if_asm)
 
-lemma "cmp_iface_name (i2 # i2s) [] \<Longrightarrow> i2 = CHR ''+''"
+lemma "iface_name_eq (i2 # i2s) [] \<Longrightarrow> i2 = CHR ''+'' \<and> i2s = []"
 proof -
-assume a: "cmp_iface_name (i2 # i2s) []"
+assume a: "iface_name_eq (i2 # i2s) []"
 { fix x1 x2
-  have "x1 = (i2 # i2s) \<Longrightarrow> x2 = [] \<Longrightarrow> cmp_iface_name x1 x2 \<Longrightarrow> i2 = CHR ''+''"
-  by(induction x1 x2 rule: cmp_iface_name.induct) (auto)
+  have "x1 = (i2 # i2s) \<Longrightarrow> x2 = [] \<Longrightarrow> iface_name_eq x1 x2 \<Longrightarrow> i2 = CHR ''+'' \<and> i2s = []"
+  by(induction x1 x2 rule: iface_name_eq.induct) (auto)
 } thus ?thesis using a by simp
 qed
 
+
+
 text{*Examples*}
-  lemma cmp_iface_name_not_trans: "\<lbrakk>i1 = ''eth0''; i2 = ''eth+''; i3 = ''eth1''\<rbrakk> \<Longrightarrow> cmp_iface_name i1 i2 \<Longrightarrow> cmp_iface_name i2 i3 \<Longrightarrow> \<not> cmp_iface_name i1 i3"
+  lemma iface_name_eq_not_trans: "\<lbrakk>i1 = ''eth0''; i2 = ''eth+''; i3 = ''eth1''\<rbrakk> \<Longrightarrow> 
+      iface_name_eq i1 i2 \<Longrightarrow> iface_name_eq i2 i3 \<Longrightarrow> \<not> iface_name_eq i1 i3"
     by(simp)
-  lemma "cmp_iface_name ''+'' i2"
-    by(induction "''+''" i2 rule: cmp_iface_name.induct) (simp_all)
-  lemma "cmp_iface_name ''eth+'' ''eth3''" by eval
-  lemma "cmp_iface_name ''eth+'' ''e+''" by eval
-  lemma "cmp_iface_name ''eth+'' ''eth_tun_foobar''" by eval
-  lemma "cmp_iface_name ''eth+'' ''eth_tun+++''" by eval
-  lemma "\<not> cmp_iface_name ''eth+'' ''wlan+''" by eval
-  lemma "cmp_iface_name ''eth1'' ''eth1''" by eval
-  lemma "\<not> cmp_iface_name ''eth1'' ''eth2''" by eval
-  text{*If the interfaces don't end in a wildcard, then @{const cmp_iface_name} is just simple equality*}
-  lemma "\<lbrakk> hd (rev i1) \<noteq> CHR ''+''; hd (rev i2) \<noteq> CHR ''+'' \<rbrakk> \<Longrightarrow> cmp_iface_name i1 i2 \<longleftrightarrow> i1 = i2"
-    apply(induction i1 i2 rule: cmp_iface_name.induct)
+  lemma "iface_name_eq ''eth+'' ''eth3''" by eval
+  lemma "iface_name_eq ''eth+'' ''e+''" by eval
+  lemma "iface_name_eq ''eth+'' ''eth_tun_foobar''" by eval
+  lemma "iface_name_eq ''eth+'' ''eth_tun+++''" by eval
+  lemma "\<not> iface_name_eq ''eth+'' ''wlan+''" by eval
+  lemma "iface_name_eq ''eth1'' ''eth1''" by eval
+  lemma "\<not> iface_name_eq ''eth1'' ''eth2''" by eval
+  lemma "iface_name_eq ''eth+'' ''eth''" by eval
+  lemma "\<not> iface_name_eq ''a'' ''b+''" by eval
+  lemma "iface_name_eq ''+'' ''''" by eval
+  lemma "iface_name_eq ''++++'' ''+''" by eval
+  text{*If the interfaces don't end in a wildcard, then @{const iface_name_eq} is just simple equality*}
+  lemma "\<lbrakk> hd (rev i1) \<noteq> CHR ''+''; hd (rev i2) \<noteq> CHR ''+'' \<rbrakk> \<Longrightarrow> iface_name_eq i1 i2 \<longleftrightarrow> i1 = i2"
+    apply(induction i1 i2 rule: iface_name_eq.induct)
     apply(simp_all)
-    apply (metis append_Nil hd_append2 list.sel(1))+
-    done
+apply (metis append_Nil hd_Cons_tl hd_append2 iface_name_eq.simps(3) iface_name_eq.simps(8) iface_name_eq_sym list.sel(1) rev_is_Nil_conv)
+by (metis append_Nil hd_Cons_tl hd_append2 iface_name_eq.simps(2) iface_name_eq.simps(7) iface_name_eq_sym list.sel(1) rev_is_Nil_conv)
+    
+
+  
+  fun iface_name_leq :: "string \<Rightarrow> string \<Rightarrow> bool" where
+    "iface_name_leq [] [] \<longleftrightarrow> True" |
+    "iface_name_leq [i1] [] \<longleftrightarrow> False" |
+    "iface_name_leq [] [i2] \<longleftrightarrow> (i2 = CHR ''+'')" |
+    "iface_name_leq [i1] [i2] \<longleftrightarrow> (i1 = i2 \<or> i2 = CHR ''+'')" |
+    "iface_name_leq (i1#i1s) (i2#i2s) \<longleftrightarrow> (i2 = CHR ''+'' \<and> i2s = []) \<or> (i1 = i2 \<and> iface_name_leq i1s i2s)" |
+    "iface_name_leq _ _ \<longleftrightarrow> False"
+
+  lemma "iface_name_leq i1 i2 \<longleftrightarrow> card {i. iface_name_eq i1 i} \<le> card {i. iface_name_eq i2 i}"
+    oops
+  lemma "iface_name_leq i1 i2 \<longleftrightarrow> iface_name_eq i1 i2 \<and> (
+            i1 = i2 \<or> 
+            iface_name_is_wildcard i2 \<and> \<not> iface_name_is_wildcard i1 \<or>
+            iface_name_is_wildcard i1 \<and> iface_name_is_wildcard i2 \<and> take ((length i2) - 1) i2 = take ((length i2) - 1) i1)"
+    apply(induction i1 i2 rule: iface_name_leq.induct)
+     apply(simp_all)
+     apply(safe)
+     apply(simp_all)
+     apply(auto elim: iface_name_leq.elims) (* OMG WTF *)
+     done
+
+
+subsection{*Matching*}
     
 fun match_iface :: "iface \<Rightarrow> string \<Rightarrow> bool" where
   "match_iface IfaceAny p_iface \<longleftrightarrow> True" |
-  "match_iface (Iface (Pos i)) p_iface \<longleftrightarrow> cmp_iface_name p_iface i" |
-  "match_iface (Iface (Neg i)) p_iface \<longleftrightarrow> \<not> cmp_iface_name p_iface i"
+  "match_iface (Iface (Pos i)) p_iface \<longleftrightarrow> iface_name_eq p_iface i" |
+  "match_iface (Iface (Neg i)) p_iface \<longleftrightarrow> \<not> iface_name_eq p_iface i"
 
+
+fun match_iface_and :: "iface \<Rightarrow> iface \<Rightarrow> iface option" where
+  "match_iface_and i IfaceAny = Some i" |
+  "match_iface_and IfaceAny i = Some i" |
+  "match_iface_and (Iface (Pos i1)) (Iface (Pos i2)) = (if iface_name_eq i1 i2 \<dots>)" (*we need the 'shorter' iface. probably we want a pseudo order on the ifaces*)
+    (*An order which is not transitive?*)
 
 end
